code/experimental/rsapss/Hacl.Impl.Bignum.Core.fst
@@ -45,30 +45,34 @@ let eq_u8 a b = FStar.UInt8.(u8_to_UInt8 a =^ u8_to_UInt8 b)
 
 (* check if input[ind] is equal to 1 *)
 val bn_is_bit_set:
-     len:bn_len
+     #len:bn_len
   -> input:lbignum len
   -> ind:size_t{v ind / 64 < v len}
   -> Stack bool
     (requires fun h -> live h input)
     (ensures  fun h0 r h1 -> modifies loc_none h0 h1 /\ h0 == h1)
 [@"c_inline"]
-let bn_is_bit_set len input ind =
+let bn_is_bit_set #len input ind =
+  [@inline_let]
   let i = ind /. 64ul in
+  [@inline_let]
   let j = ind %. 64ul in
   let tmp = input.(i) in
   let tmp = (tmp >>. j) &. u64 1 in
   eq_u64 tmp (u64 1)
 
 val bn_set_bit:
-     len:bn_len
+     #len:bn_len
   -> input:lbignum len
   -> ind:size_t{v ind / 64 < v len}
   -> Stack unit
     (requires fun h -> live h input)
     (ensures  fun h0 _ h1 -> modifies (loc input) h0 h1)
 [@"c_inline"]
-let bn_set_bit len input ind =
+let bn_set_bit #len input ind =
+  [@inline_let]
   let i = ind /. 64ul in
+  [@inline_let]
   let j = ind %. 64ul in
   let tmp = input.(i) in
   input.(i) <- tmp |. (u64 1 <<. j)
