code/experimental/rsapss/Hacl.Impl.Bignum.Shift.fst
@@ -1,0 +1,113 @@
+module Hacl.Impl.Bignum.Shift
+
+open FStar.HyperStack
+open FStar.HyperStack.ST
+open FStar.Buffer
+
+open Lib.IntTypes
+open Lib.Buffer
+open Lib.Loops
+
+open Hacl.Impl.Bignum.Core
+open Hacl.Impl.Bignum.Comparison
+open Hacl.Impl.Bignum.Addition
+
+
+
+inline_for_extraction
+let bn_tbit = u64 0x8000000000000000
+
+inline_for_extraction
+val bn_lshift1_:
+     #aLen:bn_len
+  -> a:lbignum aLen
+  -> carry:lbignum 1ul
+  -> res:lbignum aLen
+  -> Stack unit
+    (requires (fun h -> live h a /\ live h res /\ live h carry))
+    (ensures (fun h0 _ h1 -> modifies2 carry res h0 h1 /\
+                             live h1 a /\ live h1 res /\ live h1 carry))
+let bn_lshift1_ #aLen a carry res =
+  let h0 = FStar.HyperStack.ST.get() in
+  let inv h _ = live h a /\ live h carry /\ live h res /\ modifies2 carry res h0 h in
+  for 0ul aLen inv
+  (fun i ->
+    let tmp = a.(i) in
+    res.(i) <- (shift_left tmp 1ul) |. carry.(0ul);
+    carry.(size 0) <- if (eq_u64 (logand #U64 tmp bn_tbit) bn_tbit) then u64 1 else u64 0)
+
+// res = a << 1
+val bn_lshift1:
+     #aLen:bn_len
+  -> a:lbignum aLen
+  -> res:lbignum aLen
+  -> Stack unit
+    (requires (fun h -> live h a /\ live h res))
+    (ensures (fun h0 _ h1 -> modifies1 res h0 h1 /\ live h1 a /\ live h1 res))
+[@ "c_inline"]
+let bn_lshift1 #aLen a res =
+  push_frame();
+  let h0 = FStar.HyperStack.ST.get () in
+  let carry = create 1ul (uint 0) in
+  bn_lshift1_ a carry res;
+  pop_frame()
+
+inline_for_extraction
+val bn_pow2_mod_n_:
+     #aLen:bn_len
+  -> #rLen:bn_len{v aLen < v rLen}
+  -> a:lbignum aLen
+  -> p:size_t
+  -> res:lbignum rLen
+  -> Stack unit
+    (requires (fun h -> live h a /\ live h res /\ disjoint res a))
+    (ensures (fun h0 _ h1 -> modifies1 res h0 h1))
+let bn_pow2_mod_n_ #aLen #rLen a p res =
+  push_frame ();
+  let carry = create 1ul (uint 0) in
+  let h0 = FStar.HyperStack.ST.get() in
+  let inv h _ = live h carry /\ live h a /\ live h res /\ modifies2 res carry h0 h in
+  for 0ul p inv
+  (fun i ->
+    carry.(size 0) <- uint 0;
+    bn_lshift1_ res carry res;
+    (if not (bn_is_less res a) then
+      let _ = bn_sub res a res in ()));
+  pop_frame ()
+
+// res = (2 ^ p) % a
+val bn_pow2_mod_n:
+     #aLen:bn_len{v aLen + 1 < max_size_t}
+  -> aBits:size_t{v aBits / 64 <= v aLen}
+  -> a:lbignum aLen
+  -> p:size_t
+  -> res:lbignum aLen
+  -> Stack unit
+    (requires (fun h -> live h a /\ live h res /\ disjoint res a))
+    (ensures (fun h0 _ h1 -> live h1 a /\ live h1 res /\ modifies1 res h0 h1))
+[@ "c_inline"]
+let bn_pow2_mod_n #aLen aBits a p res =
+  push_frame();
+
+  let rLen = aLen +. 1ul in
+  let tmp = create rLen (u64 0) in
+
+  // Simple version. It is all very ineffective anyway, so I'll leave
+  // optimisations for later.
+  bn_set_bit tmp 0ul;
+  bn_pow2_mod_n_ a p tmp;
+
+  // Faster version
+  //if aBits >. 64ul && aBits <. p
+  //then begin
+  //  bn_set_bit tmp aBits;
+  //  //let _ = bn_sub tmp a tmp in
+  //  bn_pow2_mod_n_ a (p -. aBits) tmp
+  //end else begin
+  // // unoptimised version here
+  //end;
+
+  let tmp' = sub tmp 0ul aLen in
+  copy res tmp';
+
+  pop_frame()
